libcrux-ml-kem/src/ind_cca/instantiations.rs
@@ -106,7 +106,6 @@ macro_rules! instantiate {
 
             /// Private key validation
             #[inline(always)]
-            #[inline(always)]
             #[hax_lib::requires(fstar!("Spec.MLKEM.is_rank $K /\\
                 $SECRET_KEY_SIZE == Spec.MLKEM.v_CCA_PRIVATE_KEY_SIZE $K"))]
             pub(crate) fn validate_private_key_only<
@@ -353,6 +352,13 @@ macro_rules! instantiate {
 
                 /// Take a serialized private key and generate an unpacked key pair from it.
                 #[inline(always)]
+                #[hax_lib::requires(
+                    fstar!("Spec.MLKEM.is_rank $K /\\
+                            v_SECRET_KEY_SIZE == Spec.MLKEM.v_CCA_PRIVATE_KEY_SIZE v_K /\\
+                            v_CPA_SECRET_KEY_SIZE == Spec.MLKEM.v_CPA_PRIVATE_KEY_SIZE v_K /\\
+                            v_PUBLIC_KEY_SIZE == Spec.MLKEM.v_CPA_PUBLIC_KEY_SIZE v_K /\\
+                            v_BYTES_PER_RING_ELEMENT == Spec.MLKEM.v_RANKED_BYTES_PER_RING_ELEMENT v_K /\\
+                            v_T_AS_NTT_ENCODED_SIZE == Spec.MLKEM.v_T_AS_NTT_ENCODED_SIZE v_K"))]
                 pub(crate) fn keypair_from_private_key<
                     const K: usize,
                     const SECRET_KEY_SIZE: usize,
