libcrux-ml-kem/src/mlkem768.rs
@@ -272,6 +272,9 @@ macro_rules! instantiate {
                 }
 
                 /// Get the serialized public key.
+                #[hax_lib::requires(fstar!("(forall (i:nat). i < 3 ==>
+                        Libcrux_ml_kem.Serialize.coefficients_field_modulus_range (Seq.index 
+                            ${key_pair}.f_public_key.f_ind_cpa_public_key.f_t_as_ntt i))"))]
                 pub fn key_pair_serialized_public_key_mut(key_pair: &MlKem768KeyPairUnpacked, serialized: &mut MlKem768PublicKey) {
                     key_pair.serialized_public_key_mut::<RANKED_BYTES_PER_RING_ELEMENT_768, CPA_PKE_PUBLIC_KEY_SIZE_768>(serialized);
                 }
