libcrux-ml-kem/src/types.rs
@@ -214,7 +214,8 @@ impl<const PRIVATE_KEY_SIZE: usize, const PUBLIC_KEY_SIZE: usize>
            Seq.length ind_cpa_public_key_hash == v Libcrux_ml_kem.Constants.v_H_DIGEST_SIZE /\\
            Seq.length implicit_rejection_value == 
            Seq.length private_key - 
-             (v v_CPA_SECRET_KEY_SIZE + v v_PUBLIC_KEY_SIZE + v Libcrux_ml_kem.Constants.v_H_DIGEST_SIZE)"))]
+             (v v_CPA_SECRET_KEY_SIZE + v v_PUBLIC_KEY_SIZE + v Libcrux_ml_kem.Constants.v_H_DIGEST_SIZE)
+           "))]
 pub(crate) fn unpack_private_key<const CPA_SECRET_KEY_SIZE: usize, const PUBLIC_KEY_SIZE: usize>(
     private_key: &[u8], // len: SECRET_KEY_SIZE
 ) -> (&[u8], &[u8], &[u8], &[u8]) {
