libcrux-ml-kem/proofs/fstar/extraction/Libcrux_ml_kem.Ind_cca.Instantiations.Avx2.Unpacked.fsti
@@ -142,7 +142,14 @@ val keypair_from_private_key
             Libcrux_ml_kem.Vector.Avx2.t_SIMD256Vector)
     : Prims.Pure
       (Libcrux_ml_kem.Ind_cca.Unpacked.t_MlKemKeyPairUnpacked v_K
-          Libcrux_ml_kem.Vector.Avx2.t_SIMD256Vector) Prims.l_True (fun _ -> Prims.l_True)
+          Libcrux_ml_kem.Vector.Avx2.t_SIMD256Vector)
+      (requires
+        Spec.MLKEM.is_rank v_K /\ v_SECRET_KEY_SIZE == Spec.MLKEM.v_CCA_PRIVATE_KEY_SIZE v_K /\
+        v_CPA_SECRET_KEY_SIZE == Spec.MLKEM.v_CPA_PRIVATE_KEY_SIZE v_K /\
+        v_PUBLIC_KEY_SIZE == Spec.MLKEM.v_CPA_PUBLIC_KEY_SIZE v_K /\
+        v_BYTES_PER_RING_ELEMENT == Spec.MLKEM.v_RANKED_BYTES_PER_RING_ELEMENT v_K /\
+        v_T_AS_NTT_ENCODED_SIZE == Spec.MLKEM.v_T_AS_NTT_ENCODED_SIZE v_K)
+      (fun _ -> Prims.l_True)
 
 /// Get the unpacked public key.
 val unpack_public_key_avx2
