libcrux-ml-kem/proofs/fstar/extraction/Libcrux_ml_kem.Ind_cca.Unpacked.fst
@@ -624,17 +624,21 @@ let impl_3__serialized
           Libcrux_ml_kem.Vector.Traits.t_Operations v_Vector)
       (self: t_MlKemPublicKeyUnpacked v_K v_Vector)
      =
-  Core.Convert.f_from #(Libcrux_ml_kem.Types.t_MlKemPublicKey v_PUBLIC_KEY_SIZE)
-    #(t_Array u8 v_PUBLIC_KEY_SIZE)
-    #FStar.Tactics.Typeclasses.solve
-    (Libcrux_ml_kem.Ind_cpa.serialize_public_key v_K
-        v_RANKED_BYTES_PER_RING_ELEMENT
-        v_PUBLIC_KEY_SIZE
-        #v_Vector
-        self.f_ind_cpa_public_key.Libcrux_ml_kem.Ind_cpa.Unpacked.f_t_as_ntt
-        (self.f_ind_cpa_public_key.Libcrux_ml_kem.Ind_cpa.Unpacked.f_seed_for_A <: t_Slice u8)
-      <:
-      t_Array u8 v_PUBLIC_KEY_SIZE)
+  let result:Libcrux_ml_kem.Types.t_MlKemPublicKey v_PUBLIC_KEY_SIZE =
+    Core.Convert.f_from #(Libcrux_ml_kem.Types.t_MlKemPublicKey v_PUBLIC_KEY_SIZE)
+      #(t_Array u8 v_PUBLIC_KEY_SIZE)
+      #FStar.Tactics.Typeclasses.solve
+      (Libcrux_ml_kem.Ind_cpa.serialize_public_key v_K
+          v_RANKED_BYTES_PER_RING_ELEMENT
+          v_PUBLIC_KEY_SIZE
+          #v_Vector
+          self.f_ind_cpa_public_key.Libcrux_ml_kem.Ind_cpa.Unpacked.f_t_as_ntt
+          (self.f_ind_cpa_public_key.Libcrux_ml_kem.Ind_cpa.Unpacked.f_seed_for_A <: t_Slice u8)
+        <:
+        t_Array u8 v_PUBLIC_KEY_SIZE)
+  in
+  let _:Prims.unit = admit () (* Panic freedom *) in
+  result
 
 let impl_4__serialized_public_key
       (v_K: usize)
@@ -897,6 +901,8 @@ let impl_4__serialized_private_key
 
 #push-options "--z3rlimit 200 --ext context_pruning --z3refresh"
 
+#push-options "--admit_smt_queries true"
+
 let decapsulate
       (v_K v_SECRET_KEY_SIZE v_CPA_SECRET_KEY_SIZE v_PUBLIC_KEY_SIZE v_CIPHERTEXT_SIZE v_T_AS_NTT_ENCODED_SIZE v_C1_SIZE v_C2_SIZE v_VECTOR_U_COMPRESSION_FACTOR v_VECTOR_V_COMPRESSION_FACTOR v_C1_BLOCK_SIZE v_ETA1 v_ETA1_RANDOMNESS_SIZE v_ETA2 v_ETA2_RANDOMNESS_SIZE v_IMPLICIT_REJECTION_HASH_INPUT_SIZE:
           usize)
@@ -1026,5 +1032,7 @@ let decapsulate
   Libcrux_ml_kem.Constant_time_ops.select_shared_secret_in_constant_time shared_secret
     (implicit_rejection_shared_secret <: t_Slice u8)
     selector
+
+#pop-options
 
 #pop-options
