libcrux-ml-kem/proofs/fstar/extraction/Libcrux_ml_kem.Ind_cca.Unpacked.fsti
@@ -359,7 +359,11 @@ val impl_4__serialized_private_key_mut
       (self: t_MlKemKeyPairUnpacked v_K v_Vector)
       (serialized: Libcrux_ml_kem.Types.t_MlKemPrivateKey v_PRIVATE_KEY_SIZE)
     : Prims.Pure (Libcrux_ml_kem.Types.t_MlKemPrivateKey v_PRIVATE_KEY_SIZE)
-      Prims.l_True
+      (requires
+        Spec.MLKEM.is_rank v_K /\ v_PRIVATE_KEY_SIZE == Spec.MLKEM.v_CCA_PRIVATE_KEY_SIZE v_K /\
+        v_CPA_PRIVATE_KEY_SIZE == Spec.MLKEM.v_CPA_PRIVATE_KEY_SIZE v_K /\
+        v_PUBLIC_KEY_SIZE == Spec.MLKEM.v_CPA_PUBLIC_KEY_SIZE v_K /\
+        v_RANKED_BYTES_PER_RING_ELEMENT == Spec.MLKEM.v_RANKED_BYTES_PER_RING_ELEMENT v_K)
       (fun _ -> Prims.l_True)
 
 /// Get the serialized private key.
@@ -371,7 +375,11 @@ val impl_4__serialized_private_key
       {| i2: Libcrux_ml_kem.Vector.Traits.t_Operations v_Vector |}
       (self: t_MlKemKeyPairUnpacked v_K v_Vector)
     : Prims.Pure (Libcrux_ml_kem.Types.t_MlKemPrivateKey v_PRIVATE_KEY_SIZE)
-      Prims.l_True
+      (requires
+        Spec.MLKEM.is_rank v_K /\ v_PRIVATE_KEY_SIZE == Spec.MLKEM.v_CCA_PRIVATE_KEY_SIZE v_K /\
+        v_CPA_PRIVATE_KEY_SIZE == Spec.MLKEM.v_CPA_PRIVATE_KEY_SIZE v_K /\
+        v_PUBLIC_KEY_SIZE == Spec.MLKEM.v_CPA_PUBLIC_KEY_SIZE v_K /\
+        v_RANKED_BYTES_PER_RING_ELEMENT == Spec.MLKEM.v_RANKED_BYTES_PER_RING_ELEMENT v_K)
       (fun _ -> Prims.l_True)
 
 val decapsulate
