libcrux-ml-kem/proofs/fstar/extraction/Libcrux_ml_kem.Ind_cca.fst
@@ -61,6 +61,8 @@ let validate_private_key
 
 #pop-options
 
+#push-options "--z3rlimit 150"
+
 let serialize_kem_secret_key_mut
       (v_K v_SERIALIZED_KEY_LEN: usize)
       (#v_Hasher: Type0)
@@ -171,7 +173,43 @@ let serialize_kem_secret_key_mut
         <:
         t_Slice u8)
   in
+  let _:Prims.unit =
+    let open Spec.Utils in
+    assert ((Seq.slice serialized 0 (v #usize_inttype (Spec.MLKEM.v_CPA_PRIVATE_KEY_SIZE v_K)))
+        `Seq.equal`
+        private_key);
+    assert ((Seq.slice serialized
+            (v #usize_inttype (Spec.MLKEM.v_CPA_PRIVATE_KEY_SIZE v_K))
+            (v #usize_inttype
+                (Spec.MLKEM.v_CPA_PRIVATE_KEY_SIZE v_K +! Spec.MLKEM.v_CPA_PUBLIC_KEY_SIZE v_K)))
+        `Seq.equal`
+        public_key);
+    assert ((Seq.slice serialized
+            (v #usize_inttype
+                (Spec.MLKEM.v_CPA_PRIVATE_KEY_SIZE v_K +! Spec.MLKEM.v_CPA_PUBLIC_KEY_SIZE v_K))
+            (v #usize_inttype
+                (Spec.MLKEM.v_CPA_PRIVATE_KEY_SIZE v_K +! Spec.MLKEM.v_CPA_PUBLIC_KEY_SIZE v_K +!
+                  Libcrux_ml_kem.Constants.v_H_DIGEST_SIZE)))
+        `Seq.equal`
+        (Libcrux_ml_kem.Hash_functions.f_H #v_Hasher #v_K public_key));
+    assert (Seq.slice serialized
+          (v #usize_inttype
+              (Spec.MLKEM.v_CPA_PRIVATE_KEY_SIZE v_K +! Spec.MLKEM.v_CPA_PUBLIC_KEY_SIZE v_K +!
+                Libcrux_ml_kem.Constants.v_H_DIGEST_SIZE))
+          (v #usize_inttype
+              (Spec.MLKEM.v_CPA_PRIVATE_KEY_SIZE v_K +! Spec.MLKEM.v_CPA_PUBLIC_KEY_SIZE v_K +!
+                Libcrux_ml_kem.Constants.v_H_DIGEST_SIZE +!
+                Spec.MLKEM.v_SHARED_SECRET_SIZE)) ==
+        implicit_rejection_value);
+    lemma_slice_append_4 serialized
+      private_key
+      public_key
+      (Libcrux_ml_kem.Hash_functions.f_H #v_Hasher #v_K public_key)
+      implicit_rejection_value
+  in
   serialized
+
+#pop-options
 
 #push-options "--z3rlimit 150"
 
@@ -184,141 +222,6 @@ let serialize_kem_secret_key
       (private_key public_key implicit_rejection_value: t_Slice u8)
      =
   let out:t_Array u8 v_SERIALIZED_KEY_LEN = Rust_primitives.Hax.repeat 0uy v_SERIALIZED_KEY_LEN in
-  let pointer:usize = sz 0 in
-  let out:t_Array u8 v_SERIALIZED_KEY_LEN =
-    Rust_primitives.Hax.Monomorphized_update_at.update_at_range out
-      ({
-          Core.Ops.Range.f_start = pointer;
-          Core.Ops.Range.f_end = pointer +! (Core.Slice.impl__len #u8 private_key <: usize) <: usize
-        }
-        <:
-        Core.Ops.Range.t_Range usize)
-      (Core.Slice.impl__copy_from_slice #u8
-          (out.[ {
-                Core.Ops.Range.f_start = pointer;
-                Core.Ops.Range.f_end
-                =
-                pointer +! (Core.Slice.impl__len #u8 private_key <: usize) <: usize
-              }
-              <:
-              Core.Ops.Range.t_Range usize ]
-            <:
-            t_Slice u8)
-          private_key
-        <:
-        t_Slice u8)
-  in
-  let pointer:usize = pointer +! (Core.Slice.impl__len #u8 private_key <: usize) in
-  let out:t_Array u8 v_SERIALIZED_KEY_LEN =
-    Rust_primitives.Hax.Monomorphized_update_at.update_at_range out
-      ({
-          Core.Ops.Range.f_start = pointer;
-          Core.Ops.Range.f_end = pointer +! (Core.Slice.impl__len #u8 public_key <: usize) <: usize
-        }
-        <:
-        Core.Ops.Range.t_Range usize)
-      (Core.Slice.impl__copy_from_slice #u8
-          (out.[ {
-                Core.Ops.Range.f_start = pointer;
-                Core.Ops.Range.f_end
-                =
-                pointer +! (Core.Slice.impl__len #u8 public_key <: usize) <: usize
-              }
-              <:
-              Core.Ops.Range.t_Range usize ]
-            <:
-            t_Slice u8)
-          public_key
-        <:
-        t_Slice u8)
-  in
-  let pointer:usize = pointer +! (Core.Slice.impl__len #u8 public_key <: usize) in
-  let out:t_Array u8 v_SERIALIZED_KEY_LEN =
-    Rust_primitives.Hax.Monomorphized_update_at.update_at_range out
-      ({
-          Core.Ops.Range.f_start = pointer;
-          Core.Ops.Range.f_end = pointer +! Libcrux_ml_kem.Constants.v_H_DIGEST_SIZE <: usize
-        }
-        <:
-        Core.Ops.Range.t_Range usize)
-      (Core.Slice.impl__copy_from_slice #u8
-          (out.[ {
-                Core.Ops.Range.f_start = pointer;
-                Core.Ops.Range.f_end = pointer +! Libcrux_ml_kem.Constants.v_H_DIGEST_SIZE <: usize
-              }
-              <:
-              Core.Ops.Range.t_Range usize ]
-            <:
-            t_Slice u8)
-          (Libcrux_ml_kem.Hash_functions.f_H #v_Hasher
-              #v_K
-              #FStar.Tactics.Typeclasses.solve
-              public_key
-            <:
-            t_Slice u8)
-        <:
-        t_Slice u8)
-  in
-  let pointer:usize = pointer +! Libcrux_ml_kem.Constants.v_H_DIGEST_SIZE in
-  let out:t_Array u8 v_SERIALIZED_KEY_LEN =
-    Rust_primitives.Hax.Monomorphized_update_at.update_at_range out
-      ({
-          Core.Ops.Range.f_start = pointer;
-          Core.Ops.Range.f_end
-          =
-          pointer +! (Core.Slice.impl__len #u8 implicit_rejection_value <: usize) <: usize
-        }
-        <:
-        Core.Ops.Range.t_Range usize)
-      (Core.Slice.impl__copy_from_slice #u8
-          (out.[ {
-                Core.Ops.Range.f_start = pointer;
-                Core.Ops.Range.f_end
-                =
-                pointer +! (Core.Slice.impl__len #u8 implicit_rejection_value <: usize) <: usize
-              }
-              <:
-              Core.Ops.Range.t_Range usize ]
-            <:
-            t_Slice u8)
-          implicit_rejection_value
-        <:
-        t_Slice u8)
-  in
-  let _:Prims.unit =
-    let open Spec.Utils in
-    assert ((Seq.slice out 0 (v #usize_inttype (Spec.MLKEM.v_CPA_PRIVATE_KEY_SIZE v_K)))
-        `Seq.equal`
-        private_key);
-    assert ((Seq.slice out
-            (v #usize_inttype (Spec.MLKEM.v_CPA_PRIVATE_KEY_SIZE v_K))
-            (v #usize_inttype
-                (Spec.MLKEM.v_CPA_PRIVATE_KEY_SIZE v_K +! Spec.MLKEM.v_CPA_PUBLIC_KEY_SIZE v_K)))
-        `Seq.equal`
-        public_key);
-    assert ((Seq.slice out
-            (v #usize_inttype
-                (Spec.MLKEM.v_CPA_PRIVATE_KEY_SIZE v_K +! Spec.MLKEM.v_CPA_PUBLIC_KEY_SIZE v_K))
-            (v #usize_inttype
-                (Spec.MLKEM.v_CPA_PRIVATE_KEY_SIZE v_K +! Spec.MLKEM.v_CPA_PUBLIC_KEY_SIZE v_K +!
-                  Libcrux_ml_kem.Constants.v_H_DIGEST_SIZE)))
-        `Seq.equal`
-        (Libcrux_ml_kem.Hash_functions.f_H #v_Hasher #v_K public_key));
-    assert (Seq.slice out
-          (v #usize_inttype
-              (Spec.MLKEM.v_CPA_PRIVATE_KEY_SIZE v_K +! Spec.MLKEM.v_CPA_PUBLIC_KEY_SIZE v_K +!
-                Libcrux_ml_kem.Constants.v_H_DIGEST_SIZE))
-          (v #usize_inttype
-              (Spec.MLKEM.v_CPA_PRIVATE_KEY_SIZE v_K +! Spec.MLKEM.v_CPA_PUBLIC_KEY_SIZE v_K +!
-                Libcrux_ml_kem.Constants.v_H_DIGEST_SIZE +!
-                Spec.MLKEM.v_SHARED_SECRET_SIZE)) ==
-        implicit_rejection_value);
-    lemma_slice_append_4 out
-      private_key
-      public_key
-      (Libcrux_ml_kem.Hash_functions.f_H #v_Hasher #v_K public_key)
-      implicit_rejection_value
-  in
   let out:t_Array u8 v_SERIALIZED_KEY_LEN =
     serialize_kem_secret_key_mut v_K
       v_SERIALIZED_KEY_LEN
@@ -332,7 +235,7 @@ let serialize_kem_secret_key
 
 #pop-options
 
-#push-options "--z3rlimit 150"
+#push-options "--z3rlimit 300"
 
 let encapsulate
       (v_K v_CIPHERTEXT_SIZE v_PUBLIC_KEY_SIZE v_T_AS_NTT_ENCODED_SIZE v_C1_SIZE v_C2_SIZE v_VECTOR_U_COMPRESSION_FACTOR v_VECTOR_V_COMPRESSION_FACTOR v_C1_BLOCK_SIZE v_ETA1 v_ETA1_RANDOMNESS_SIZE v_ETA2 v_ETA2_RANDOMNESS_SIZE:
@@ -417,9 +320,13 @@ let encapsulate
       shared_secret
       ciphertext
   in
-  ciphertext, shared_secret_array
-  <:
-  (Libcrux_ml_kem.Types.t_MlKemCiphertext v_CIPHERTEXT_SIZE & t_Array u8 (sz 32))
+  let result:(Libcrux_ml_kem.Types.t_MlKemCiphertext v_CIPHERTEXT_SIZE & t_Array u8 (sz 32)) =
+    ciphertext, shared_secret_array
+    <:
+    (Libcrux_ml_kem.Types.t_MlKemCiphertext v_CIPHERTEXT_SIZE & t_Array u8 (sz 32))
+  in
+  let _:Prims.unit = admit () (* Panic freedom *) in
+  result
 
 #pop-options
 
@@ -453,6 +360,8 @@ let validate_public_key
         t_Slice u8)
   in
   public_key =. public_key_serialized
+
+#push-options "--z3rlimit 300"
 
 let generate_keypair
       (v_K v_CPA_PRIVATE_KEY_SIZE v_PRIVATE_KEY_SIZE v_PUBLIC_KEY_SIZE v_RANKED_BYTES_PER_RING_ELEMENT v_ETA1 v_ETA1_RANDOMNESS_SIZE:
@@ -503,15 +412,21 @@ let generate_keypair
       #FStar.Tactics.Typeclasses.solve
       secret_key_serialized
   in
-  Libcrux_ml_kem.Types.impl_21__from v_PRIVATE_KEY_SIZE
-    v_PUBLIC_KEY_SIZE
-    private_key
-    (Core.Convert.f_from #(Libcrux_ml_kem.Types.t_MlKemPublicKey v_PUBLIC_KEY_SIZE)
-        #(t_Array u8 v_PUBLIC_KEY_SIZE)
-        #FStar.Tactics.Typeclasses.solve
-        public_key
-      <:
-      Libcrux_ml_kem.Types.t_MlKemPublicKey v_PUBLIC_KEY_SIZE)
+  let result:Libcrux_ml_kem.Types.t_MlKemKeyPair v_PRIVATE_KEY_SIZE v_PUBLIC_KEY_SIZE =
+    Libcrux_ml_kem.Types.impl_21__from v_PRIVATE_KEY_SIZE
+      v_PUBLIC_KEY_SIZE
+      private_key
+      (Core.Convert.f_from #(Libcrux_ml_kem.Types.t_MlKemPublicKey v_PUBLIC_KEY_SIZE)
+          #(t_Array u8 v_PUBLIC_KEY_SIZE)
+          #FStar.Tactics.Typeclasses.solve
+          public_key
+        <:
+        Libcrux_ml_kem.Types.t_MlKemPublicKey v_PUBLIC_KEY_SIZE)
+  in
+  let _:Prims.unit = admit () (* Panic freedom *) in
+  result
+
+#pop-options
 
 #push-options "--z3rlimit 500"
 
@@ -677,15 +592,20 @@ let decapsulate
       shared_secret
       ciphertext
   in
-  Libcrux_ml_kem.Constant_time_ops.compare_ciphertexts_select_shared_secret_in_constant_time (Core.Convert.f_as_ref
-        #(Libcrux_ml_kem.Types.t_MlKemCiphertext v_CIPHERTEXT_SIZE)
-        #(t_Slice u8)
-        #FStar.Tactics.Typeclasses.solve
-        ciphertext
-      <:
-      t_Slice u8)
-    (expected_ciphertext <: t_Slice u8)
-    (shared_secret <: t_Slice u8)
-    (implicit_rejection_shared_secret <: t_Slice u8)
+  let shared_secret:t_Array u8 (sz 32) =
+    Libcrux_ml_kem.Constant_time_ops.compare_ciphertexts_select_shared_secret_in_constant_time (Core.Convert.f_as_ref
+          #(Libcrux_ml_kem.Types.t_MlKemCiphertext v_CIPHERTEXT_SIZE)
+          #(t_Slice u8)
+          #FStar.Tactics.Typeclasses.solve
+          ciphertext
+        <:
+        t_Slice u8)
+      (expected_ciphertext <: t_Slice u8)
+      (shared_secret <: t_Slice u8)
+      (implicit_rejection_shared_secret <: t_Slice u8)
+  in
+  let result:t_Array u8 (sz 32) = shared_secret in
+  let _:Prims.unit = admit () (* Panic freedom *) in
+  result
 
 #pop-options
